src/HOL/Imperative_HOL/ex/Imperative_Reverse.thy
@@ -8,14 +8,12 @@ theory Imperative_Reverse
 imports Imperative_HOL Subarray
 begin
 
-hide_const (open) swap rev
-
 fun swap :: "'a\<Colon>heap array \<Rightarrow> nat \<Rightarrow> nat \<Rightarrow> unit Heap" where
   "swap a i j = do {
-     x \<leftarrow> nth a i;
-     y \<leftarrow> nth a j;
-     upd i y a;
-     upd j x a;
+     x \<leftarrow> Array.nth a i;
+     y \<leftarrow> Array.nth a j;
+     Array.upd i y a;
+     Array.upd j x a;
      return ()
    }"
 
@@ -25,9 +23,6 @@ fun rev :: "'a\<Colon>heap array \<Rightarrow> nat \<Rightarrow> nat \<Rightarro
      rev a (i + 1) (j - 1)
    }
    else return ())"
-
-notation (output) swap ("swap")
-notation (output) rev ("rev")
 
 declare swap.simps [simp del] rev.simps [simp del]
 
